generic

src/TL.lean
@@ -1,3 +1,4 @@
+import data.finset
 namespace TT
 
 inductive type : Type
@@ -45,13 +46,13 @@ notation `⁎` := star    -- input \asterisk
 notation `⊤` := top     --       \top
 notation `⊥` := bot     -- input \bot
 infixr ` ⟹ `:60 := imp -- input \==>
-infixr ` ⊓ ` :70 := and -- input \glb or \sqcap
-infixr ` ⊔ ` :59 := or  -- input \lub or ⊔
+infixr ` ⋀ ` :70 := and -- input \glb or \sqcap
+infixr ` ⋁ ` :59 := or  -- input \lub or ⋁
 
 def not (p : term) := p ⟹ ⊥
 prefix `∼`:max := not -- input \~, the ASCII character ~ has too low precedence
 
-def biimp (p q: term) := (p ⟹ q) ⊓ (q ⟹ p)
+def biimp (p q: term) := (p ⟹ q) ⋀ (q ⟹ p)
 infix ` ⇔ `:60 := biimp -- input \<=>
 
 infix ∈ := elem
@@ -82,8 +83,8 @@ inductive WF : context → term → type → Prop
 | star {Γ}           : WF Γ term.star 𝟙
 | top  {Γ}           : WF Γ term.top Ω
 | bot  {Γ}           : WF Γ term.bot Ω
-| and  {Γ e₁ e₂}     : WF Γ e₁ Ω → WF Γ e₁ Ω → WF Γ (e₁ ⊓ e₂) Ω
-| or   {Γ e₁ e₂}     : WF Γ e₁ Ω → WF Γ e₁ Ω → WF Γ (e₁ ⊔ e₂) Ω
+| and  {Γ e₁ e₂}     : WF Γ e₁ Ω → WF Γ e₁ Ω → WF Γ (e₁ ⋀ e₂) Ω
+| or   {Γ e₁ e₂}     : WF Γ e₁ Ω → WF Γ e₁ Ω → WF Γ (e₁ ⋁ e₂) Ω
 | imp  {Γ e₁ e₂}     : WF Γ e₁ Ω → WF Γ e₁ Ω → WF Γ (e₁ ⟹ e₂) Ω
 | var  {Γ n A}       : list.nth Γ n = some A → WF Γ (var n) A
 | comp {Γ e A}       : WF (A::Γ) e Ω → WF Γ ⟦e⟧ (𝒫 A)
@@ -92,28 +93,51 @@ inductive WF : context → term → type → Prop
 | elem {Γ e₁ e₂ A}   : WF Γ e₁ A → WF Γ e₂ (𝒫 A) → WF Γ (e₁ ∈ e₂) Ω
 | prod {Γ e₁ e₂ A B} : WF Γ e₁ A → WF Γ e₂ B → WF Γ (prod e₁ e₂) (A ×× B)
 
-def subst_nth (b:term) : ℕ → term → term
-| n star       := star
-| n top        := top
-| n bot        := bot
-| n (p ⊓ q)    := (subst_nth n p) ⊓ (subst_nth n q)
-| n (p ⊔ q)    := (subst_nth n p) ⊔ (subst_nth n q)
-| n (p ⟹ q)  := (subst_nth n p) ⟹ (subst_nth n q)
-| n (var m)    := if n=m then b else var m
-| n ⟦φ⟧        := ⟦subst_nth (n+1) φ⟧
-| n (∀' φ)     := ∀' (subst_nth (n+1) φ)
-| n (∃' φ)     := ∃' (subst_nth (n+1) φ)
-| n (a ∈ α)    := (subst_nth n a) ∈ (subst_nth n α)
-| n (prod a b) := prod (subst_nth n a) (subst_nth n b)
+lemma WF_and_left {Γ p q} : WF Γ (p ⋀ q) Ω → WF Γ p Ω := sorry
+lemma WF_and_right {Γ p q} : WF Γ (p ⋀ q) Ω → WF Γ q Ω := sorry
+lemma WF_or_left {Γ p q} : WF Γ (p ⋁ q) Ω → WF Γ p Ω := sorry
+lemma WF_or_right {Γ p q} : WF Γ (p ⋁ q) Ω → WF Γ q Ω := sorry
+lemma WF_imp_left {Γ p q} : WF Γ (p ⟹ q) Ω → WF Γ p Ω := sorry
+lemma WF_imp_right {Γ p q} : WF Γ (p ⟹ q) Ω → WF Γ q Ω := sorry
 
-def subst (b:term):= subst_nth b 0
+#check @WF.and
+
+def lift (d : ℕ): ℕ → term → term
+| k star       := star
+| k top        := top
+| k bot        := bot
+| k (p ⋀ q)    := (lift k p) ⋀ (lift k q)
+| k (p ⋁ q)    := (lift k p) ⋁ (lift k q)
+| k (p ⟹ q)    := (lift k p) ⟹ (lift k q)
+| k (var m)    := if m≥k then var (m+d) else var m
+| k ⟦φ⟧         :=    ⟦lift (k+1) φ⟧
+| k (∀' φ)     := ∀' lift (k+1) φ
+| k (∃' φ)     := ∃' lift (k+1) φ
+| k (a ∈ α)    := (lift k a) ∈ (lift k α)
+| k (prod a b) := prod (lift k a) (lift k b)
+
+def subst_nth : term → ℕ → term → term
+| b n star       := star
+| b n top        := top
+| b n bot        := bot
+| b n (p ⋀ q)    := (subst_nth b n p) ⋀ (subst_nth b n q)
+| b n (p ⋁ q)    := (subst_nth b n p) ⋁ (subst_nth b n q)
+| b n (p ⟹ q)  := (subst_nth b n p) ⟹ (subst_nth b n q)
+| b n (var m)    := if n=m then b else var m
+| b n ⟦φ⟧        :=     ⟦subst_nth (lift 1 0 b) (n+1) φ⟧
+| b n (∀' φ)     := ∀' (subst_nth (lift 1 0 b) (n+1) φ)
+| b n (∃' φ)     := ∃' (subst_nth (lift 1 0 b) (n+1) φ)
+| b n (a ∈ α)    := (subst_nth b n a) ∈ (subst_nth b n α)
+| b n (prod a c) := prod (subst_nth b n a) (subst_nth b n c)
+
+def subst (b:term) := subst_nth b 0
 
 def remap_vars : Π k : ℕ, (ℕ → ℕ) → term → term
 | k σ top        := top
 | k σ star       := star
 | k σ bot        := bot
-| k σ (p ⊓ q)   := (remap_vars k σ p) ⊓ (remap_vars k σ q)
-| k σ (p ⊔ q)   := (remap_vars k σ p) ⊔ (remap_vars k σ q)
+| k σ (p ⋀ q)   := (remap_vars k σ p) ⋀ (remap_vars k σ q)
+| k σ (p ⋁ q)   := (remap_vars k σ p) ⋁ (remap_vars k σ q)
 | k σ (p ⟹ q)  := (remap_vars k σ p) ⟹ (remap_vars k σ q)
 | k σ (var m)    := var (σ (m+k))
 | k σ ⟦φ⟧         := ⟦remap_vars (k+1) σ φ⟧
@@ -128,24 +152,25 @@ inductive proof : context → term → term → Prop
 | vac        {Γ φ}     : WF Γ φ Ω → proof Γ φ term.top
 | abs        {Γ φ}     : WF Γ φ Ω → proof Γ term.bot φ
 | cut        {Γ φ ψ γ} : proof Γ φ ψ → proof Γ ψ γ → proof Γ φ γ
-| and_intro  {Γ p q r} : proof Γ p q → proof Γ p r → proof Γ p (q ⊓ r)  
-| and_left   {Γ p q r} : proof Γ p (q ⊓ r) → proof Γ p q
-| and_right  {Γ p q r} : proof Γ p (q ⊓ r) → proof Γ p r
-| or_intro   {Γ p q r} : proof Γ p r → proof Γ q r → proof Γ (p ⊔ q) r  
-| or_left    {Γ p q r} : proof Γ (p ⊔ q) r → proof Γ p r
-| or_right   {Γ p q r} : proof Γ (p ⊔ q) r → proof Γ q r
-| imp_to_and {Γ p q r} : proof Γ p (q ⟹ r) → proof Γ (p ⊓ q) r
-| and_to_imp {Γ p q r} : proof Γ (p ⊓ q) r → proof Γ p (q ⟹ r)
+| and_intro  {Γ p q r} : proof Γ p q → proof Γ p r → proof Γ p (q ⋀ r)  
+| and_left   {Γ p q r} : proof Γ p (q ⋀ r) → proof Γ p q
+| and_right  {Γ p q r} : proof Γ p (q ⋀ r) → proof Γ p r
+| or_intro   {Γ p q r} : proof Γ p r → proof Γ q r → proof Γ (p ⋁ q) r  
+| or_left    {Γ p q r} : proof Γ (p ⋁ q) r → proof Γ p r
+| or_right   {Γ p q r} : proof Γ (p ⋁ q) r → proof Γ q r
+| imp_to_and {Γ p q r} : proof Γ p (q ⟹ r) → proof Γ (p ⋀ q) r
+| and_to_imp {Γ p q r} : proof Γ (p ⋀ q) r → proof Γ p (q ⟹ r)
+| add_var    {Γ φ ψ B} : proof Γ φ ψ → proof (B :: Γ) φ ψ
 
 | apply    {Γ φ ψ b B} :
     WF Γ b B
     → proof (B::Γ) φ ψ
-    → proof Γ (subst b φ) (subst b ψ) -- can free vars in b become bound?? (bad)
+    → proof Γ (subst b φ) (subst b ψ)
 
-| all_elim   {Γ p φ B} : proof (B::Γ) p (all φ) → proof Γ p φ
-| all_intro  {Γ p φ B} : proof Γ p φ → proof (B::Γ) p (∀' φ)
-| ex_elim    {Γ p φ B} : proof (B::Γ) p (∃' φ) → proof Γ p φ
-| ex_intro   {Γ p φ B} : proof Γ p φ → proof (B::Γ) p (∃' φ)
+| all_elim   {Γ p φ B} : proof Γ p (∀' φ) → proof (B::Γ) p φ
+| all_intro  {Γ p φ B} : proof (B::Γ) p φ → proof Γ p (∀' φ)
+| ex_elim    {Γ p φ B} : proof Γ p (∃' φ) → proof (B::Γ) p φ
+| ex_intro   {Γ p φ B} : proof (B::Γ) p φ → proof Γ p (∃' φ)
 
 | comp       {Γ φ A}   :
     WF (A::A::Γ) φ Ω
@@ -162,16 +187,54 @@ inductive proof : context → term → term → Prop
 
 | prod_distinct_rep    :
     proof [] ⊤
-      ∀' ∀' ∀' ∀' (prod <3> <1> ≃ prod <2> <0>) ⟹ (<3> ≃ <2> ⊓ <1> ≃ <0>)
+      ∀' ∀' ∀' ∀' (prod <3> <1> ≃ prod <2> <0>) ⟹ (<3> ≃ <2> ⋀ <1> ≃ <0>)
 
 example : proof [] ⊤ ⊤ := proof.axm WF.top
 
 lemma proof_WF {Γ : context} {P Q: term} : WF Γ P Ω → proof Γ P Q → WF Γ Q Ω := sorry
+-- begin
+-- intros wfP prf,
+-- induction prf,
+-- case proof.axm {exact wfP},
+-- case proof.vac {exact WF.top},
+-- case proof.abs {exact prf_a},
+-- case proof.cut {sorry},
+-- end
 
 variables p q r : term
 
-example {Γ : context}  : proof Γ ⊤ (q ⟹ r) → proof Γ q r := sorry
+example {Γ : context} : proof Γ ⊤ (q ⟹ r) → proof Γ q r := sorry
+-- begin
+-- intro h₁,
+-- apply @proof.cut Γ q (⊤ ⋀ q) r,
+-- apply proof.and_intro,
+-- apply proof.vac,
+-- apply WF_imp_left,
+-- end
 
-def FV {Γ : context} {A : type} (a : term): WF Γ a A → context := λ _, Γ
+-- example {Γ : context} : proof Γ ⊤ (p ⋀ q) → proof Γ ⊤ (q ⋀ p) :=
+-- λ h₁, proof.and_intro (proof.and_right h₁) (proof.and_left h₁)
+example {Γ : context} : proof Γ ⊤ (p ⋀ q) → proof Γ ⊤ (q ⋀ p) :=
+begin
+intro h₁,
+apply proof.and_intro,
+exact proof.and_right h₁,
+exact proof.and_left h₁,
+end
+
+def FV {Γ : context} {A : type} (a : term): WF Γ a A → finset ℕ := sorry
+-- | _ star       := ∅
+-- | _ top        := ∅
+-- | _ bot        := ∅
+-- | _ (p ⋀ q)    := (FV k p) ∪ (FV k q)
+-- | _ (p ⋁ q)    := (FV k p) ∪ (FV k q)
+-- | _ (p ⟹ q)    := (FV k p) ⟹ (FV k q)
+-- | _ (var m)    := if m≥k then var (m+d) else var m
+-- | _ ⟦φ⟧         :=    ⟦FV (k+1) φ⟧
+-- | _ (∀' φ)     := ∀' FV (k+1) φ
+-- | _ (∃' φ)     := ∃' FV (k+1) φ
+-- | _ (a ∈ α)    := (FV k a) ∈ (FV k α)
+-- | _ (prod a b) := prod (FV k a) (FV k b)
+
 
 end TT
